iris/ProofSysChdir.v
@@ -902,7 +902,7 @@ Section ProofSysChdirBody.
     (k < NINODE)%nat ->
     (ic_sleeplocks cn -∗
      ∃ gil gisl : gname,
-       is_sleeplock gil gisl (i_lock (ientry k)) "inode"%string (ic_tok cn k)
+       is_sleeplock_gen gil gisl (i_lock (ientry k)) "inode"%string (ic_tok cn k) (slh_tok (icfg_isl k))
      : iProp Σ).
   Proof.
     iIntros (Hk) "H". rewrite /ic_sleeplocks.
