iris/SpecIunlockput.v
@@ -172,9 +172,9 @@ Definition wp_iunlockput_sconf_body
   itable_inv -∗
   ic_escrow cn gfs gi cov logstart k -∗
   ireg_inv gi gfs inodestart nib -∗
-  is_sleeplock gil gisl (i_lock ip) "inode"%string (ic_tok cn k) -∗
+  is_sleeplock_gen gil gisl (i_lock ip) "inode"%string (ic_tok cn k) (slh_tok (icfg_isl k)) -∗
   (* ---- THE HOLDER'S BUNDLE (SpecIunlock's precondition) ---- *)
-  sleeplocked gisl -∗
+  sleeplocked_q gisl s -∗
   sl_pid (i_lock ip) ↦₄ pidv -∗
   ic_deposit cn k (DepShr s dev inum gy) -∗
   i_dev ip ↦₄{DfracOwn (1/2)} dev -∗
@@ -302,9 +302,9 @@ Definition wp_iunlockput_gen_body
   itable_inv -∗
   ic_escrow cn gfs gi cov logstart k -∗
   ireg_inv gi gfs inodestart nib -∗
-  is_sleeplock gil gisl (i_lock ip) "inode"%string (ic_tok cn k) -∗
+  is_sleeplock_gen gil gisl (i_lock ip) "inode"%string (ic_tok cn k) (slh_tok (icfg_isl k)) -∗
   (* ---- THE HOLDER'S BUNDLE (SpecIunlock's precondition) ---- *)
-  sleeplocked gisl -∗
+  sleeplocked_q gisl s -∗
   sl_pid (i_lock ip) ↦₄ pidv -∗
   ic_deposit cn k (DepShr s dev inum gy) -∗
   i_dev ip ↦₄{DfracOwn (1/2)} dev -∗
